{
  "@context": {
    "schema": "http://schema.org/",
    "rdf": "http://www.w3.org/1999/02/22-rdf-syntax-ns#",
    "rdfs": "http://www.w3.org/2000/01/rdf-schema#",
    "outbreaktest": "http://discovery.biothings.io/view/"
  },
  "@graph": [
    {
      "@id": "outbreaktest:CitationObject",
      "@type": "rdfs:Class",
      "rdfs:comment": "A citation object for a resource which is cited by the subject (ie- is a derivative of the subject), related to the subject, or from which the subject was based on (ie- is derived from).",
      "rdfs:label": "CitationObject",
      "rdfs:subClassOf": {
        "@id": "schema:CreativeWork"
      },
      "$validation": {
        "$schema": "http://json-schema.org/draft-07/schema#",
        "type": "object",
        "properties": {
          "citeText": {
            "description": "The bibliographic citation for the referenced resource as is provided",
            "type": "string"
          },
          "versionDate": {
            "description": "The version date of the resource used at the time of the creation of the citation as certain resources (protocols, datasets) may change frequently over time.",
            "format": "date",
            "type": "string"
          },
          "pmid": {
            "description": "A pubmed identifier if available",
            "type": "string"
          },
          "doi": {
            "description": "A doi if available",
            "type": "string"
          },
          "type": {
            "description": "The type of resource",
            "enum": [
              "Dataset",
              "Publication",
              "ClinicalTrial",
              "Analysis",
              "Protocol",
              "SoftwareApplication",
              "CreativeWork"
            ]
          },
          "identifier": {
            "description": "The identifier property represents any kind of identifier for any kind of <a class=\"localLink\" href=\"http://schema.org/Thing\">Thing</a>, such as ISBNs, GTIN codes, UUIDs etc. Schema.org provides dedicated properties for representing many of these, either as textual strings or as URL (URI) links. See <a href=\"/docs/datamodel.html#identifierBg\">background notes</a> for more details.",
            "type": "string"
          },
          "name": {
            "description": "The name of the item.",
            "type": "string"
          },
          "url": {
            "description": "URL of the item.",
            "type": "string",
            "format": "uri"
          }
        },
        "required": [
          "name"
        ]
      }
    },
    {
      "@id": "outbreaktest:citeText",
      "@type": "rdfs:Property",
      "rdfs:comment": "The bibliographic citation for the referenced resource as is provided",
      "rdfs:label": "citeText",
      "schema:domainIncludes": {
        "@id": "outbreaktest:CitationObject"
      },
      "schema:rangeIncludes": [
        {
          "@id": "schema:Text"
        }
      ]
    },
    {
      "@id": "outbreaktest:versionDate",
      "@type": "rdfs:Property",
      "rdfs:comment": "The version date of the resource used at the time of the creation of the citation as certain resources (protocols, datasets) may change frequently over time.",
      "rdfs:label": "versionDate",
      "schema:domainIncludes": {
        "@id": "outbreaktest:CitationObject"
      },
      "schema:rangeIncludes": [
        {
          "@id": "schema:Date"
        }
      ]
    },
    {
      "@id": "outbreaktest:pmid",
      "@type": "rdfs:Property",
      "rdfs:comment": "A pubmed identifier if available",
      "rdfs:label": "pmid",
      "schema:domainIncludes": {
        "@id": "outbreaktest:CitationObject"
      },
      "schema:rangeIncludes": [
        {
          "@id": "schema:Text"
        }
      ]
    },
    {
      "@id": "outbreaktest:doi",
      "@type": "rdfs:Property",
      "rdfs:comment": "A doi if available",
      "rdfs:label": "doi",
      "schema:domainIncludes": {
        "@id": "outbreaktest:CitationObject"
      },
      "schema:rangeIncludes": [
        {
          "@id": "schema:Text"
        }
      ]
    },
    {
      "@id": "outbreaktest:type",
      "@type": "rdfs:Property",
      "rdfs:comment": "The type of resource",
      "rdfs:label": "type",
      "schema:domainIncludes": {
        "@id": "outbreaktest:CitationObject"
      },
      "schema:rangeIncludes": [
        {
          "@id": "schema:Text"
        }
      ]
    }
  ]
}