{
  "@context": {
    "schema": "http://schema.org/",
    "rdf": "http://www.w3.org/1999/02/22-rdf-syntax-ns#",
    "rdfs": "http://www.w3.org/2000/01/rdf-schema#",
    "bioschemastest": "http://discovery.biothings.io/view/bioschemastest/"
  },
  "@graph": [
    {
      "@id": "bioschemastest:ComputationalWorkflow",
      "@type": "rdfs:Class",
      "rdfs:comment": "A computational workflow consists of an orchestrated and repeatable pattern of activity enabled by the systematic organization of resources into processes that transform materials, provide services, or process information (source Wikipedia.org). It is executed by a computational process and is thus distinct from laboratory or business workflows. version 1.0-RELEASE",
      "rdfs:label": "ComputationalWorkflow",
      "rdfs:subClassOf": {
        "@id": "schema:SoftwareSourceCode"
      },
      "$validation": {
        "$schema": "http://json-schema.org/draft-07/schema#",
        "type": "object",
        "properties": {
          "input": {
            "description": "An input required to use the computational workflow (eg. Excel spreadsheet, BAM file)",
            "oneOf": [
              {
                "$ref": "#/definitions/formalParameter"
              },
              {
                "type": "array",
                "items": {
                  "$ref": "#/definitions/formalParameter"
                }
              }
            ]
          },
          "output": {
            "description": "An output produced by the workflow",
            "oneOf": [
              {
                "$ref": "#/definitions/formalParameter"
              },
              {
                "type": "array",
                "items": {
                  "$ref": "#/definitions/formalParameter"
                }
              }
            ]
          },
          "creativeWorkStatus": {
            "description": "The status of a creative work in terms of its stage in a lifecycle. Example terms include Incomplete, Draft, Published, Obsolete. Some organizations define a set of terms for the stages of their publication lifecycle.",
            "anyOf": [
              {
                "type": "string"
              },
              {
                "type": "array",
                "items": {
                  "type": "string"
                }
              },
              {
                "$ref": "#/definitions/definedTerm"
              },
              {
                "type": "array",
                "items": {
                  "$ref": "#/definitions/definedTerm"
                }
              }
            ]
          },
          "documentation": {
            "description": "Documentation describing the ComputationalWorkflow and its use.",
            "anyOf": [
              {
                "type": "string",
                "format": "uri"
              },
              {
                "type": "array",
                "items": {
                  "type": "string",
                  "format": "uri"
                }
              },
              {
                "$ref": "#/definitions/creativeWork"
              },
              {
                "type": "array",
                "items": {
                  "$ref": "#/definitions/creativeWork"
                }
              }
            ]
          },
          "funding": {
            "description": "The funding for the workflow",
            "oneOf": [
              {
                "$ref": "#/definitions/grant"
              },
              {
                "type": "array",
                "items": {
                  "$ref": "#/definitions/grant"
                }
              }
            ]
          },
          "maintainer": {
            "description": " maintainer of a Dataset, software package (SoftwareApplication), or other Project. A maintainer is a Person or Organization that manages contributions to, and/or publication of, some (typically complex) artifact. It is common for distributions of software and data to be based on \u201cupstream\u201d sources. When maintainer is applied to a specific version of something e.g. a particular version or packaging of a Dataset, it is always possible that the upstream source has a different maintainer. The isBasedOn property can be used to indicate such relationships between datasets to make the different maintenance roles clear. Similarly in the case of software, a package may have dedicated maintainers working on integration into software distributions such as Ubuntu, as well as upstream maintainers of the underlying work.",
            "anyOf": [
              {
                "$ref": "#/definitions/person"
              },
              {
                "type": "array",
                "items": {
                  "$ref": "#/definitions/person"
                }
              },
              {
                "$ref": "#/definitions/organization"
              },
              {
                "type": "array",
                "items": {
                  "$ref": "#/definitions/organization"
                }
              }
            ]
          },
          "softwareRequirements": {
            "description": "Renaming schema.org/requirements as softwareRequirements. Component dependency requirements for application. This includes runtime environments and shared libraries that are not included in the application distribution package, but required to run the application (Examples: DirectX, Java or .NET runtime). Supersedes requirements. ",
            "oneOf": [
              {
                "type": "string",
                "format": "uri"
              },
              {
                "type": "array",
                "items": {
                  "type": "string",
                  "format": "uri"
                }
              },
              {
                "type": "string"
              },
              {
                "type": "array",
                "items": {
                  "type": "string"
                }
              }
            ]
          },
          "targetProduct": {
            "description": "Target Operating System / Product to which the code applies.  If applies to several versions, just the product name can be used.",
            "oneOf": [
              {
                "$ref": "#/definitions/softwareApplication"
              },
              {
                "type": "array",
                "items": {
                  "$ref": "#/definitions/softwareApplication"
                }
              }
            ]
          },
          "programmingLanguage": {
            "description": "The computer programming language.",
            "anyOf": [
              {
                "type": "string"
              },
              {
                "type": "array",
                "items": {
                  "type": "string"
                }
              },
              {
                "$ref": "#/definitions/computerLanguage"
              },
              {
                "type": "array",
                "items": {
                  "$ref": "#/definitions/computerLanguage"
                }
              }
            ]
          },
          "runtimePlatform": {
            "description": "Runtime platform or script interpreter dependencies (Example - Java v1, Python2.3, .Net Framework 3.0).",
            "oneOf": [
              {
                "type": "string"
              },
              {
                "type": "array",
                "items": {
                  "type": "string"
                }
              }
            ]
          },
          "description": {
            "description": "A description of the item.",
            "type": "string"
          },
          "name": {
            "description": "The name of the item.",
            "type": "string"
          },
          "url": {
            "description": "URL of the item.",
            "type": "string",
            "format": "uri"
          },
          "citation": {
            "description": "A citation or reference to another creative work, such as another publication, web page, scholarly article, etc.",
            "anyOf": [
              {
                "type": "string"
              },
              {
                "type": "array",
                "items": {
                  "type": "string"
                }
              },
              {
                "$ref": "#/definitions/creativeWork"
              },
              {
                "type": "array",
                "items": {
                  "$ref": "#/definitions/creativeWork"
                }
              }
            ]
          },
          "contributor": {
            "description": "A secondary contributor to the CreativeWork or Event.",
            "anyOf": [
              {
                "$ref": "#/definitions/person"
              },
              {
                "type": "array",
                "items": {
                  "$ref": "#/definitions/person"
                }
              },
              {
                "$ref": "#/definitions/organization"
              },
              {
                "type": "array",
                "items": {
                  "$ref": "#/definitions/organization"
                }
              }
            ]
          },
          "creator": {
            "description": "The creator/author of this CreativeWork. This is the same as the Author property for CreativeWork.",
            "anyOf": [
              {
                "$ref": "#/definitions/person"
              },
              {
                "type": "array",
                "items": {
                  "$ref": "#/definitions/person"
                }
              },
              {
                "$ref": "#/definitions/organization"
              },
              {
                "type": "array",
                "items": {
                  "$ref": "#/definitions/organization"
                }
              }
            ]
          },
          "dateCreated": {
            "description": "The date on which the CreativeWork was created or the item was added to a DataFeed.",
            "format": "date",
            "type": "string"
          },
          "hasPart": {
            "description": "Indicates an item or CreativeWork that is part of this item, or CreativeWork (in some sense).",
            "oneOf": [
              {
                "$ref": "#/definitions/creativeWork"
              },
              {
                "type": "array",
                "items": {
                  "$ref": "#/definitions/creativeWork"
                }
              }
            ]
          },
          "isBasedOn": {
            "description": "A resource from which this work is derived or from which it is a modification or adaption.",
            "oneOf": [
              {
                "$ref": "#/definitions/product"
              },
              {
                "$ref": "#/definitions/creativeWork"
              },
              {
                "type": "string",
                "format": "uri"
              }
            ]
          },
          "keywords": {
            "description": "Keywords or tags used to describe this content. Multiple entries in a keywords list are typically delimited by commas.",
            "oneOf": [
              {
                "type": "string"
              },
              {
                "type": "array",
                "items": {
                  "type": "string"
                }
              }
            ]
          },
          "license": {
            "description": "A license document that applies to this content, typically indicated by URL.",
            "anyOf": [
              {
                "type": "string",
                "format": "uri"
              },
              {
                "type": "array",
                "items": {
                  "type": "string",
                  "format": "uri"
                }
              },
              {
                "$ref": "#/definitions/creativeWork"
              },
              {
                "type": "array",
                "items": {
                  "$ref": "#/definitions/creativeWork"
                }
              }
            ]
          },
          "producer": {
            "description": "The person or organization who produced the work (e.g. music album, movie, tv/radio series etc.).",
            "anyOf": [
              {
                "$ref": "#/definitions/person"
              },
              {
                "type": "array",
                "items": {
                  "$ref": "#/definitions/person"
                }
              },
              {
                "$ref": "#/definitions/organization"
              },
              {
                "type": "array",
                "items": {
                  "$ref": "#/definitions/organization"
                }
              }
            ]
          },
          "publisher": {
            "description": "The publisher of the creative work.",
            "anyOf": [
              {
                "$ref": "#/definitions/person"
              },
              {
                "type": "array",
                "items": {
                  "$ref": "#/definitions/person"
                }
              },
              {
                "$ref": "#/definitions/organization"
              },
              {
                "type": "array",
                "items": {
                  "$ref": "#/definitions/organization"
                }
              }
            ]
          },
          "sdPublisher": {
            "description": "Indicates the party responsible for generating and publishing the current structured data markup, typically in cases where the structured data is derived automatically from existing published content but published on a different site. For example, student projects and open data initiatives often re-publish existing content with more explicitly structured metadata. The\n<a class=\"localLink\" href=\"http://schema.org/sdPublisher\">sdPublisher</a> property helps make such practices more explicit.",
            "anyOf": [
              {
                "$ref": "#/definitions/person"
              },
              {
                "type": "array",
                "items": {
                  "$ref": "#/definitions/person"
                }
              },
              {
                "$ref": "#/definitions/organization"
              },
              {
                "type": "array",
                "items": {
                  "$ref": "#/definitions/organization"
                }
              }
            ]
          },
          "version": {
            "description": "The version of the CreativeWork embodied by a specified resource.",
            "oneOf": [
              {
                "type": "string"
              },
              {
                "type": "number"
              }
            ]
          }
        },
        "required": [
          "input",
          "output",
          "programmingLanguage",
          "name",
          "url",
          "creator",
          "dateCreated",
          "license",
          "sdPublisher",
          "version"
        ],
        "definitions": {
          "formalParameter": {
            "@type": "bioschemas:FormalParameter",
            "type": "object",
            "properties": {
              "name": {
                "type": "string"
              },
              "identifier": {
                "type": "string"
              },
              "url": {
                "type": "string",
                "format": "uri"
              }
            },
            "required": []
          },
          "grant": {
            "@type": "Grant",
            "type": "object",
            "properties": {
              "name": {
                "type": "string"
              },
              "url": {
                "type": "string",
                "format": "uri"
              },
              "sponsor": {
                "oneOf": [
                  {
                    "$ref": "#/definitions/organization"
                  },
                  {
                    "$ref": "#/definitions/person"
                  }
                ]
              },
              "identifier": {
                "type": "string"
              }
            },
            "required": [
              "name"
            ]
          },
          "person": {
            "@type": "Person",
            "type": "object",
            "properties": {
              "name": {
                "type": "string"
              },
              "url": {
                "type": "string",
                "format": "uri"
              },
              "affiliation": {
                "$ref": "#/definitions/organization"
              }
            },
            "required": [
              "name"
            ]
          },
          "softwareApplication": {
            "@type": "SoftwareApplication",
            "type": "object",
            "properties": {
              "name": {
                "type": "string"
              },
              "url": {
                "type": "string",
                "format": "uri"
              }
            },
            "required": []
          },
          "creativeWork": {
            "@type": "CreativeWork",
            "type": "object",
            "properties": {
              "name": {
                "type": "string"
              },
              "identifier": {
                "type": "string"
              },
              "url": {
                "type": "string",
                "format": "uri"
              }
            },
            "required": []
          },
          "product": {
            "@type": "Product",
            "type": "object",
            "properties": {
              "name": {
                "type": "string"
              },
              "identifier": {
                "type": "string"
              },
              "url": {
                "type": "string",
                "format": "uri"
              }
            },
            "required": []
          }
        }
      }
    },
    {
      "@id": "bioschemastest:input",
      "@type": "rdf:Property",
      "rdfs:comment": "An input required to use the computational workflow (eg. Excel spreadsheet, BAM file)",
      "rdfs:label": "input",
      "schema:domainIncludes": {
        "@id": "bioschemastest:ComputationalWorkflow"
      },
      "schema:rangeIncludes": [
        {
          "@id": "bioschemas:FormalParameter"
        }
      ]
    },
    {
      "@id": "bioschemastest:output",
      "@type": "rdf:Property",
      "rdfs:comment": "An output produced by the workflow",
      "rdfs:label": "output",
      "schema:domainIncludes": {
        "@id": "bioschemastest:ComputationalWorkflow"
      },
      "schema:rangeIncludes": [
        {
          "@id": "bioschemas:FormalParameter"
        }
      ]
    },
    {
      "@id": "bioschemastest:creativeWorkStatus",
      "@type": "rdf:Property",
      "rdfs:comment": "The status of a creative work in terms of its stage in a lifecycle. Example terms include Incomplete, Draft, Published, Obsolete. Some organizations define a set of terms for the stages of their publication lifecycle.",
      "rdfs:label": "creativeWorkStatus",
      "schema:domainIncludes": {
        "@id": "bioschemastest:ComputationalWorkflow"
      },
      "schema:rangeIncludes": [
        {
          "@id": "schema:Text"
        },
        {
          "@id": "schema:DefinedTerm"
        }
      ]
    },
    {
      "@id": "bioschemastest:documentation",
      "@type": "rdf:Property",
      "rdfs:comment": "Documentation describing the ComputationalWorkflow and its use.",
      "rdfs:label": "documentation",
      "schema:domainIncludes": {
        "@id": "bioschemastest:ComputationalWorkflow"
      },
      "schema:rangeIncludes": [
        {
          "@id": "schema:CreativeWork"
        },
        {
          "@id": "schema:URL"
        }
      ]
    },
    {
      "@id": "bioschemastest:funding",
      "@type": "rdf:Property",
      "rdfs:comment": "The funding for the workflow",
      "rdfs:label": "funding",
      "schema:domainIncludes": {
        "@id": "bioschemastest:ComputationalWorkflow"
      },
      "schema:rangeIncludes": [
        {
          "@id": "schema:Grant"
        }
      ]
    },
    {
      "@id": "bioschemastest:maintainer",
      "@type": "rdf:Property",
      "rdfs:comment": " maintainer of a Dataset, software package (SoftwareApplication), or other Project. A maintainer is a Person or Organization that manages contributions to, and/or publication of, some (typically complex) artifact. It is common for distributions of software and data to be based on \u201cupstream\u201d sources. When maintainer is applied to a specific version of something e.g. a particular version or packaging of a Dataset, it is always possible that the upstream source has a different maintainer. The isBasedOn property can be used to indicate such relationships between datasets to make the different maintenance roles clear. Similarly in the case of software, a package may have dedicated maintainers working on integration into software distributions such as Ubuntu, as well as upstream maintainers of the underlying work.",
      "rdfs:label": "maintainer",
      "schema:domainIncludes": {
        "@id": "bioschemastest:ComputationalWorkflow"
      },
      "schema:rangeIncludes": [
        {
          "@id": "schema:Person"
        },
        {
          "@id": "schema:Organization"
        }
      ]
    },
    {
      "@id": "bioschemastest:softwareRequirements",
      "@type": "rdf:Property",
      "rdfs:comment": "Renaming schema.org/requirements as softwareRequirements. Component dependency requirements for application. This includes runtime environments and shared libraries that are not included in the application distribution package, but required to run the application (Examples: DirectX, Java or .NET runtime). Supersedes requirements. ",
      "rdfs:label": "softwareRequirements",
      "schema:domainIncludes": {
        "@id": "bioschemastest:ComputationalWorkflow"
      },
      "schema:rangeIncludes": [
        {
          "@id": "schema:Text"
        },
        {
          "@id": "schema:URL"
        }
      ]
    }
  ]
}