{
  "@context": {
    "schema": "http://schema.org/",
    "rdf": "http://www.w3.org/1999/02/22-rdf-syntax-ns#",
    "rdfs": "http://www.w3.org/2000/01/rdf-schema#",
    "outbreaktest": "http://discovery.biothings.io/view/"
  },
  "@graph": [
    {
      "@id": "outbreaktest:Outcome",
      "@type": "rdfs:Class",
      "rdfs:comment": "This is the schema for describing a Clinical Trial/Study Outcome for inclusion in  outbreak.info Resources",
      "rdfs:label": "Outcome",
      "rdfs:subClassOf": {
        "@id": "schema:Thing"
      },
      "$validation": {
        "$schema": "http://json-schema.org/draft-07/schema#",
        "type": "object",
        "properties": {
          "outcomeMeasure": {
            "description": "The outcome measure for the study",
            "type": "string"
          },
          "outcomeTimeFrame": {
            "description": "The specific time point(s) and overall duration of evaluation must be specified in this section",
            "type": "string"
          },
          "outcomeType": {
            "description": "The classification of the outcome measure as either primary, secondary, or exploratory",
            "oneOf": [
              {
                "type": "string",
                "enum": [
                  "primary",
                  "secondary",
                  "exploratory"
                ]
              },
              {
                "type": "string"
              }
            ]
          }
        },
        "required": []
      }
    },
    {
      "@id": "outbreaktest:outcomeMeasure",
      "@type": "rdfs:Property",
      "rdfs:comment": "The outcome measure for the study",
      "rdfs:label": "outcomeMeasure",
      "schema:domainIncludes": {
        "@id": "outbreaktest:Outcome"
      },
      "schema:rangeIncludes": [
        {
          "@id": "schema:Text"
        }
      ]
    },
    {
      "@id": "outbreaktest:outcomeTimeFrame",
      "@type": "rdfs:Property",
      "rdfs:comment": "The specific time point(s) and overall duration of evaluation must be specified in this section",
      "rdfs:label": "outcomeTimeFrame",
      "schema:domainIncludes": {
        "@id": "outbreaktest:Outcome"
      },
      "schema:rangeIncludes": [
        {
          "@id": "schema:Duration"
        },
        {
          "@id": "schema:Text"
        }
      ]
    },
    {
      "@id": "outbreaktest:outcomeType",
      "@type": "rdfs:Property",
      "rdfs:comment": "The classification of the outcome measure as either primary, secondary, or exploratory",
      "rdfs:label": "outcomeType",
      "schema:domainIncludes": {
        "@id": "outbreaktest:Outcome"
      },
      "schema:rangeIncludes": [
        {
          "@id": "schema:Text"
        }
      ]
    }
  ]
}