{
  "@context": {
    "schema": "http://schema.org/",
    "rdf": "http://www.w3.org/1999/02/22-rdf-syntax-ns#",
    "rdfs": "http://www.w3.org/2000/01/rdf-schema#",
    "outbreaktest": "http://discovery.biothings.io/view/"
  },
  "@graph": [
    {
      "@id": "outbreaktest:StudyEvent",
      "@type": "rdfs:Class",
      "rdfs:comment": "This is the schema for describing StudyEvents, a class that describes categorical events in Clinical Trials added to outbreak.info",
      "rdfs:label": "StudyEvent",
      "rdfs:subClassOf": {
        "@id": "schema:Event"
      },
      "$validation": {
        "$schema": "http://json-schema.org/draft-07/schema#",
        "type": "object",
        "properties": {
          "studyEventType": {
            "description": "Type of the event status such as StudyStart, PrimaryCompletion, Completion, StudyFirstSubmit, StudyFirstSubmitQC, LastUpdateSubmit",
            "oneOf": [
              {
                "type": "string",
                "enum": [
                  "StudyStart",
                  "PrimaryCompletion",
                  "Completion",
                  "StudyFirstSubmit",
                  "StudyFirstSubmitQC",
                  "LastUpdateSubmit"
                ]
              },
              {
                "type": "array",
                "items": {
                  "type": "string",
                  "enum": [
                    "StudyStart",
                    "PrimaryCompletion",
                    "Completion",
                    "StudyFirstSubmit",
                    "StudyFirstSubmitQC",
                    "LastUpdateSubmit"
                  ]
                }
              }
            ]
          },
          "studyEventDate": {
            "description": "The corresponding/actual date of the study event (ie- the StartDate, Primary CompletionDate, CompletionDate, StudyFirstSubmitDate, StudyFirstSubmitQCDate, LastUpdateSubmitDate)",
            "format": "date",
            "type": "string"
          },
          "studyEventDateType": {
            "description": "the type of date provided (actual, anticipated, or estimated)",
            "oneOf": [
              {
                "type": "string",
                "enum": [
                  "actual",
                  "anticipated",
                  "estimated"
                ]
              },
              {
                "type": "array",
                "items": {
                  "type": "string",
                  "enum": [
                    "actual",
                    "anticipated",
                    "estimated"
                  ]
                }
              }
            ]
          }
        },
        "required": []
      }
    },
    {
      "@id": "outbreaktest:studyEventType",
      "@type": "rdfs:Property",
      "rdfs:comment": "Type of the event status such as StudyStart, PrimaryCompletion, Completion, StudyFirstSubmit, StudyFirstSubmitQC, LastUpdateSubmit",
      "rdfs:label": "studyEventType",
      "schema:domainIncludes": {
        "@id": "outbreaktest:StudyEvent"
      },
      "schema:rangeIncludes": [
        {
          "@id": "schema:Text"
        }
      ]
    },
    {
      "@id": "outbreaktest:studyEventDate",
      "@type": "rdfs:Property",
      "rdfs:comment": "The corresponding/actual date of the study event (ie- the StartDate, Primary CompletionDate, CompletionDate, StudyFirstSubmitDate, StudyFirstSubmitQCDate, LastUpdateSubmitDate)",
      "rdfs:label": "studyEventDate",
      "schema:domainIncludes": {
        "@id": "outbreaktest:StudyEvent"
      },
      "schema:rangeIncludes": [
        {
          "@id": "schema:Date"
        }
      ]
    },
    {
      "@id": "outbreaktest:studyEventDateType",
      "@type": "rdfs:Property",
      "rdfs:comment": "the type of date provided (actual, anticipated, or estimated)",
      "rdfs:label": "studyEventDateType",
      "schema:domainIncludes": {
        "@id": "outbreaktest:StudyEvent"
      },
      "schema:rangeIncludes": [
        {
          "@id": "schema:Text"
        }
      ]
    }
  ]
}