{
  "@context": {
    "schema": "http://schema.org/",
    "rdf": "http://www.w3.org/1999/02/22-rdf-syntax-ns#",
    "rdfs": "http://www.w3.org/2000/01/rdf-schema#",
    "outbreaktest": "http://discovery.biothings.io/view/"
  },
  "@graph": [
    {
      "@id": "outbreaktest:StudyLocation",
      "@type": "rdfs:Class",
      "rdfs:comment": "This is the schema for describing Clinical Trial/Study locations for inclusion in outbreak.info Resources",
      "rdfs:label": "StudyLocation",
      "rdfs:subClassOf": {
        "@id": "schema:Place"
      },
      "$validation": {
        "$schema": "http://json-schema.org/draft-07/schema#",
        "type": "object",
        "properties": {
          "studyLocation": {
            "description": "The location of the study",
            "@type": "Place",
            "type": "object",
            "properties": {
              "name": {
                "type": "string"
              }
            },
            "required": [
              "name"
            ]
          },
          "studyLocationCity": {
            "description": "The city in which the facility used for the study is located",
            "@type": "City",
            "type": "object",
            "properties": {
              "name": {
                "type": "string"
              }
            },
            "required": [
              "name"
            ]
          },
          "studyLocationState": {
            "description": "The state or province in which the facility used for the study is located",
            "@type": "State",
            "type": "object",
            "properties": {
              "name": {
                "type": "string"
              }
            },
            "required": [
              "name"
            ]
          },
          "studyLocationCountry": {
            "description": "The country in which the facility used for the study is located",
            "@type": "Country",
            "type": "object",
            "properties": {
              "name": {
                "type": "string"
              }
            },
            "required": [
              "name"
            ]
          },
          "studyLocationStatus": {
            "description": "The recruitment status of the study at the specific study site",
            "type": "string"
          }
        },
        "required": []
      }
    },
    {
      "@id": "outbreaktest:studyLocation",
      "@type": "rdfs:Property",
      "rdfs:comment": "The location of the study",
      "rdfs:label": "studyLocation",
      "schema:domainIncludes": {
        "@id": "outbreaktest:StudyLocation"
      },
      "schema:rangeIncludes": [
        {
          "@id": "schema:Place"
        }
      ]
    },
    {
      "@id": "outbreaktest:studyLocationCity",
      "@type": "rdfs:Property",
      "rdfs:comment": "The city in which the facility used for the study is located",
      "rdfs:label": "studyLocationCity",
      "schema:domainIncludes": {
        "@id": "outbreaktest:StudyLocation"
      },
      "schema:rangeIncludes": [
        {
          "@id": "schema:City"
        }
      ]
    },
    {
      "@id": "outbreaktest:studyLocationState",
      "@type": "rdfs:Property",
      "rdfs:comment": "The state or province in which the facility used for the study is located",
      "rdfs:label": "studyLocationState",
      "schema:domainIncludes": {
        "@id": "outbreaktest:StudyLocation"
      },
      "schema:rangeIncludes": [
        {
          "@id": "schema:State"
        }
      ]
    },
    {
      "@id": "outbreaktest:studyLocationCountry",
      "@type": "rdfs:Property",
      "rdfs:comment": "The country in which the facility used for the study is located",
      "rdfs:label": "studyLocationCountry",
      "schema:domainIncludes": {
        "@id": "outbreaktest:StudyLocation"
      },
      "schema:rangeIncludes": [
        {
          "@id": "schema:Country"
        }
      ]
    },
    {
      "@id": "outbreaktest:studyLocationStatus",
      "@type": "rdfs:Property",
      "rdfs:comment": "The recruitment status of the study at the specific study site",
      "rdfs:label": "studyLocationStatus",
      "schema:domainIncludes": {
        "@id": "outbreaktest:StudyLocation"
      },
      "schema:rangeIncludes": [
        {
          "@id": "schema:Text"
        }
      ]
    }
  ]
}