{
  "@context": {
    "schema": "http://schema.org/",
    "rdf": "http://www.w3.org/1999/02/22-rdf-syntax-ns#",
    "rdfs": "http://www.w3.org/2000/01/rdf-schema#",
    "outbreaktest": "http://discovery.biothings.io/view/"
  },
  "@graph": [
    {
      "@id": "outbreaktest:StudyDesign",
      "@type": "rdfs:Class",
      "rdfs:comment": "This is the schema for describing the study design of a clinical trial/study for inclusion into outbreak.info resources",
      "rdfs:label": "StudyDesign",
      "rdfs:subClassOf": {
        "@id": "schema:MedicalStudy"
      },
      "$validation": {
        "$schema": "http://json-schema.org/draft-07/schema#",
        "type": "object",
        "properties": {
          "studyType": {
            "description": "Type of human study, can be subtypes of observational study or interventional studies and may include the temporal relationship of observation period to time of participant enrollment.",
            "oneOf": [
              {
                "type": "string"
              },
              {
                "type": "array",
                "items": {
                  "type": "string"
                }
              }
            ]
          },
          "phase": {
            "description": "Stage or phase of the study in the U.S. if applicable",
            "oneOf": [
              {
                "type": "string"
              },
              {
                "type": "array",
                "items": {
                  "type": "string"
                }
              }
            ]
          },
          "phaseNumber": {
            "description": "The number of the phase or stage of the study",
            "oneOf": [
              {
                "type": "string"
              },
              {
                "type": "array",
                "items": {
                  "type": "string"
                }
              }
            ]
          },
          "designAllocation": {
            "description": "The method by which the study participants were allocated into groups",
            "type": "string"
          },
          "designModel": {
            "description": "The general design of the strategy for assigning interventions to participants in a clinical intervention study OR the general design of the strategy for identifying and following up with participants during an observational study",
            "oneOf": [
              {
                "type": "string"
              },
              {
                "type": "array",
                "items": {
                  "type": "string"
                }
              }
            ]
          },
          "designPrimaryPurpose": {
            "description": "The primary purpose of the study",
            "oneOf": [
              {
                "type": "string"
              },
              {
                "type": "array",
                "items": {
                  "type": "string"
                }
              }
            ]
          },
          "designWhoMasked": {
            "description": "The people who do not know which participants have been assigned to which interventions",
            "oneOf": [
              {
                "type": "string"
              },
              {
                "type": "array",
                "items": {
                  "type": "string"
                }
              }
            ]
          },
          "designStudyText": {
            "description": "String description of the study design if structured information not available",
            "type": "string"
          }
        },
        "required": []
      }
    },
    {
      "@id": "outbreaktest:studyType",
      "@type": "rdfs:Property",
      "rdfs:comment": "Type of human study, can be subtypes of observational study or interventional studies and may include the temporal relationship of observation period to time of participant enrollment.",
      "rdfs:label": "studyType",
      "schema:domainIncludes": {
        "@id": "outbreaktest:StudyDesign"
      },
      "schema:rangeIncludes": [
        {
          "@id": "schema:Text"
        }
      ]
    },
    {
      "@id": "outbreaktest:phase",
      "@type": "rdfs:Property",
      "rdfs:comment": "Stage or phase of the study in the U.S. if applicable",
      "rdfs:label": "phase",
      "schema:domainIncludes": {
        "@id": "outbreaktest:StudyDesign"
      },
      "schema:rangeIncludes": [
        {
          "@id": "schema:Text"
        }
      ]
    },
    {
      "@id": "outbreaktest:phaseNumber",
      "@type": "rdfs:Property",
      "rdfs:comment": "The number of the phase or stage of the study",
      "rdfs:label": "phaseNumber",
      "schema:domainIncludes": {
        "@id": "outbreaktest:StudyDesign"
      },
      "schema:rangeIncludes": [
        {
          "@id": "schema:Number"
        }
      ]
    },
    {
      "@id": "outbreaktest:designAllocation",
      "@type": "rdfs:Property",
      "rdfs:comment": "The method by which the study participants were allocated into groups",
      "rdfs:label": "designAllocation",
      "schema:domainIncludes": {
        "@id": "outbreaktest:StudyDesign"
      },
      "schema:rangeIncludes": [
        {
          "@id": "schema:Text"
        }
      ]
    },
    {
      "@id": "outbreaktest:designModel",
      "@type": "rdfs:Property",
      "rdfs:comment": "The general design of the strategy for assigning interventions to participants in a clinical intervention study OR the general design of the strategy for identifying and following up with participants during an observational study",
      "rdfs:label": "designModel",
      "schema:domainIncludes": {
        "@id": "outbreaktest:StudyDesign"
      },
      "schema:rangeIncludes": [
        {
          "@id": "schema:Text"
        }
      ]
    },
    {
      "@id": "outbreaktest:designPrimaryPurpose",
      "@type": "rdfs:Property",
      "rdfs:comment": "The primary purpose of the study",
      "rdfs:label": "designPrimaryPurpose",
      "schema:domainIncludes": {
        "@id": "outbreaktest:StudyDesign"
      },
      "schema:rangeIncludes": [
        {
          "@id": "schema:Text"
        }
      ]
    },
    {
      "@id": "outbreaktest:designWhoMasked",
      "@type": "rdfs:Property",
      "rdfs:comment": "The people who do not know which participants have been assigned to which interventions",
      "rdfs:label": "designWhoMasked",
      "schema:domainIncludes": {
        "@id": "outbreaktest:StudyDesign"
      },
      "schema:rangeIncludes": [
        {
          "@id": "schema:Text"
        }
      ]
    },
    {
      "@id": "outbreaktest:designStudyText",
      "@type": "rdfs:Property",
      "rdfs:comment": "String description of the study design if structured information not available",
      "rdfs:label": "designStudyText",
      "schema:domainIncludes": {
        "@id": "outbreaktest:StudyDesign"
      },
      "schema:rangeIncludes": [
        {
          "@id": "schema:Text"
        }
      ]
    }
  ]
}