{
  "@context": {
    "schema": "http://schema.org/",
    "rdf": "http://www.w3.org/1999/02/22-rdf-syntax-ns#",
    "rdfs": "http://www.w3.org/2000/01/rdf-schema#",
    "outbreaktest": "http://discovery.biothings.io/view/"
  },
  "@graph": [
    {
      "@id": "outbreaktest:StudyStatus",
      "@type": "rdfs:Class",
      "rdfs:comment": "This is the schema for describing the status of a ClinicalTrial resource in outbreak.info",
      "rdfs:label": "StudyStatus",
      "rdfs:subClassOf": {
        "@id": "schema:MedicalStudy"
      },
      "$validation": {
        "$schema": "http://json-schema.org/draft-07/schema#",
        "type": "object",
        "properties": {
          "statusExpandedAccess": {
            "description": "Flag for whether or not the study has expanded Access status",
            "type": "string"
          },
          "statusDate": {
            "description": "The date that the status was verified. Equivalent to NCT's StatusVerifiedDate",
            "format": "date",
            "type": "string"
          },
          "enrollmentCount": {
            "description": "The number of participants enrolled in the study",
            "type": "string"
          },
          "enrollmentType": {
            "description": "The type of estimation used to determine the enrollmentCount (actual counts, target size, etc.)",
            "oneOf": [
              {
                "type": "string",
                "enum": [
                  "actual counts",
                  "target size"
                ]
              },
              {
                "type": "string"
              }
            ]
          },
          "whyStopped": {
            "description": "A brief explanation of the reason(s) why such clinical study was stopped (for a clinical study that is Suspended, Terminated, or Withdrawn prior to its planned completion as anticipated by the protocol)",
            "type": "string"
          },
          "status": {
            "description": "The status of the study (enumerated).",
            "type": "string"
          }
        },
        "required": []
      }
    },
    {
      "@id": "outbreaktest:statusExpandedAccess",
      "@type": "rdfs:Property",
      "rdfs:comment": "Flag for whether or not the study has expanded Access status",
      "rdfs:label": "statusExpandedAccess",
      "schema:domainIncludes": {
        "@id": "outbreaktest:StudyStatus"
      },
      "schema:rangeIncludes": [
        {
          "@id": "schema:Boolean"
        }
      ]
    },
    {
      "@id": "outbreaktest:statusDate",
      "@type": "rdfs:Property",
      "rdfs:comment": "The date that the status was verified. Equivalent to NCT's StatusVerifiedDate",
      "rdfs:label": "statusDate",
      "schema:domainIncludes": {
        "@id": "outbreaktest:StudyStatus"
      },
      "schema:rangeIncludes": [
        {
          "@id": "schema:Date"
        }
      ]
    },
    {
      "@id": "outbreaktest:enrollmentCount",
      "@type": "rdfs:Property",
      "rdfs:comment": "The number of participants enrolled in the study",
      "rdfs:label": "enrollmentCount",
      "schema:domainIncludes": {
        "@id": "outbreaktest:StudyStatus"
      },
      "schema:rangeIncludes": [
        {
          "@id": "schema:Number"
        }
      ]
    },
    {
      "@id": "outbreaktest:enrollmentType",
      "@type": "rdfs:Property",
      "rdfs:comment": "The type of estimation used to determine the enrollmentCount (actual counts, target size, etc.)",
      "rdfs:label": "enrollmentType",
      "schema:domainIncludes": {
        "@id": "outbreaktest:StudyStatus"
      },
      "schema:rangeIncludes": [
        {
          "@id": "schema:Text"
        }
      ]
    },
    {
      "@id": "outbreaktest:whyStopped",
      "@type": "rdfs:Property",
      "rdfs:comment": "A brief explanation of the reason(s) why such clinical study was stopped (for a clinical study that is Suspended, Terminated, or Withdrawn prior to its planned completion as anticipated by the protocol)",
      "rdfs:label": "whyStopped",
      "schema:domainIncludes": {
        "@id": "outbreaktest:StudyStatus"
      },
      "schema:rangeIncludes": [
        {
          "@id": "schema:Text"
        }
      ]
    }
  ]
}